maybe use fin instead?

lib/SystemF.v
@@ -16,8 +16,10 @@ Inductive LE (n : nat) : nat -> Set :=
   n ≤ S m
 where "x ≤ y" := (LE x y) : type_scope.
 
+Equations Derive NoConfusion NoConfusionHom Subterm for nat.
+
 Derive Signature for LE.
-Equations Derive NoConfusion (*NoConfusionHom*) (*Subterm*) for LE.
+Equations Derive NoConfusion for LE.
 
 Equations S_LE : forall {n m}, n ≤ m -> S n ≤ S m :=
   S_LE (LE_n n) := LE_n (S n);
@@ -90,19 +92,16 @@ Next Obligation.
 Defined.
 
 Equations Derive Subterm for LE.
-   
 
 Lemma LE_eq : forall {n m : nat} (h h' : n ≤ m), h = h'.
 Proof.
-  intros n m; generalize dependent n.
-  induction m as [| m ih]; intros n h h'.
-  - depelim h; depelim h'; reflexivity.
-  - destruct n as [| n].
-    + depelim h; depelim h'.
-      pose proof ih 0 h h' as H; rewrite H; reflexivity.
-    + pose proof S_impl_LE h as H.
-      pose proof S_impl_LE h' as H'.
-      pose
+  intros n m h h';
+    induction h; depelim h'.
+  - rewrite LE_n_eq; reflexivity.
+  - exfalso; apply not_S_n_LE_n in h'; inv h'.
+  - clear IHh; exfalso; apply not_S_n_LE_n in h; inv h.
+  - f_equal; auto.
+Defined.
     
 Equations ext_LE : forall {Δ₁ Δ₂ : nat},
     (forall n, n ≤ Δ₁ -> n ≤ Δ₂) -> forall {n : nat}, n ≤ S Δ₁ -> n ≤ S Δ₂ :=
@@ -112,6 +111,12 @@ Equations ext_LE : forall {Δ₁ Δ₂ : nat},
 Definition LT (n m : nat) : Set := S n ≤ m.
 Notation "x '`<' y"
   := (LT x y) (at level 80, no associativity) : type_scope.
+
+Lemma LT_eq : forall {n m : nat} (h h' : n `< m), h = h'.
+Proof.
+  intros n m.
+  refine LE_eq.
+Defined.
 
 Definition S_LT {n m : nat} : n `< m -> S n `< S m := S_LE.
 
@@ -178,7 +183,8 @@ Equations type_eq_dec : forall {Δ : nat} (τ ρ : type Δ), {τ = ρ} + {τ <> 
       | left _     => left _ } };
   type_eq_dec _ _ := right _.
 Next Obligation.
-
+  f_equal. apply LT_eq.
+Defined.
 
 Equations rename_type : forall {Δ₁ Δ₂ : nat},
     (forall n, n `< Δ₁ -> n `< Δ₂) -> type Δ₁ -> type Δ₂ :=
@@ -201,6 +207,35 @@ Equations subs_type : forall {Δ₁ Δ₂ : nat},
   subs_type σ (τ → τ')%ty := (subs_type σ τ → subs_type σ τ')%ty;
   subs_type σ (∀ τ)%ty    := (∀ subs_type (exts_type σ) τ)%ty.
 
+Definition S_type_suber : forall {Δ₁ Δ₂ : nat},
+    (forall n, n `< Δ₁ -> type Δ₂) -> forall n, n `< S Δ₁ -> type (S Δ₂).
+Proof.
+  intros Δ₁ Δ₂ f n h.
+  unfold "`<" in *.
+  depelim h.
+  - admit.
+  - eapply S_type, f, h.
+Admitted.
+
+Lemma S_type_subs : forall {Δ₁ Δ₂ : nat}
+    (σ : forall n, n `< Δ₁ -> type Δ₂) (τ : type Δ₁),
+    S_type (subs_type σ τ) = subs_type (S_type_suber σ) (S_type τ).
+Proof.
+  intros Δ₁ Δ₂ σ τ.
+  funelim (subs_type σ τ).
+  - rewrite S_type_equation_1.
+    do 2 rewrite subs_type_equation_1.
+    admit. (* maybe use [fin nat]? *)
+  - rewrite S_type_equation_2.
+    do 2 rewrite subs_type_equation_2.
+    rewrite S_type_equation_2.
+    rewrite H. admit. (* lemma for [exts] *)
+  - rewrite S_type_equation_3.
+    do 2 rewrite subs_type_equation_3.
+    rewrite S_type_equation_3.
+    rewrite H, H0. reflexivity.
+Admitted.
+
 Definition sub_type : forall {Δ : nat}, type (S Δ) -> type Δ -> type Δ.
 Proof.
   intros Δ body arg.
@@ -214,6 +249,11 @@ Defined.
 
 Notation "x '`[[' y ']]'"
   := (sub_type x y) (at level 12, no associativity) : ty_scope.
+
+Lemma S_type_sub : forall {Δ : nat} (τ : type (S Δ)) (τ' : type Δ),
+    S_type (τ `[[ τ' ]])%ty = (S_type τ `[[ S_type τ' ]])%ty.
+Proof.
+Admitted.
 
 Reserved Notation "Γ '⊢' τ" (at level 80, no associativity).
 
@@ -238,6 +278,7 @@ where "Γ '⊢' τ" := (term Γ τ).
 
 Derive Signature for term.
 Equations Derive NoConfusion (* NoConfusionHom *) (*Subterm*) for term.
+(*Equations Derive Subterm for term.*)
 
 Definition lookup : forall {Δ : nat} {Γ : list (type Δ)} {n : nat},
     n `< len Γ -> type Δ.
@@ -298,7 +339,32 @@ Notation "t '⦗' τ '⦘'"
   := (TypApp _ _ τ t)
        (at level 39, left associativity) : term_scope.
 
-Definition has_map : forall (A B : Set) (f : A -> B) (l : list A) b,
+Definition has_map : forall {A B : Set} (f : A -> B) {l a},
+    Has a l -> Has (f a) (map f l).
+Proof.
+  intros A B f l; induction l as [| h t ih];
+    intros a H; cbn in *.
+  - apply H.
+  - destruct H as [H | H]; subst.
+    + left; reflexivity.
+    + right; apply ih,H.
+Defined.
+
+Equations S_term : forall {Δ : nat} {Γ : list (type Δ)} {τ : type Δ},
+    Γ ⊢ τ -> map S_type Γ ⊢ S_type τ :=
+  S_term (Id _ _ h)     := Id _ _ (has_map S_type h);
+  S_term (`λ t)%term    := (`λ S_term t)%term;
+  S_term (t₁ ⋅ t₂)%term := (S_term t₁ ⋅ S_term t₂)%term;
+  S_term (Λ t)%term     := (Λ S_term t)%term;
+  S_term (t ⦗ τ ⦘)%term := _.
+Next Obligation.
+  pose proof S_term _ _ _ t as St.
+  rewrite S_type_equation_2 in St.
+  pose proof (St ⦗ S_type τ ⦘)%term as t'.
+  rewrite S_type_sub. exact t'.
+Defined.
+
+Definition map_has : forall (A B : Set) (f : A -> B) (l : list A) b,
     Has b (map f l) -> {a : A & f a = b & Has a l}.
 Proof.
   intros A B f l.
@@ -314,31 +380,45 @@ Definition S_Renamer : forall {Δ : nat} {Γ₁ Γ₂ : list (type Δ)},
     (forall τ : type Δ, Has τ Γ₁ -> Has τ Γ₂) ->
     forall τ : type (S Δ), Has τ (map S_type Γ₁) -> Has τ (map S_type Γ₂).
 Proof.
-  intros Δ Γ₁.
-  induction Γ₁ as [| τ₁ Γ₁ ih]; intros [| τ₂ Γ₂] f τ h; cbn in *.
-  - inv h.
-  - inv h.
-  - destruct h as [h | h]; subst.
-    + specialize f with (τ := τ₁).
-      apply f. left; reflexivity.
-    + apply has_map in h as [τ' τ'eq hasτ'].
-      specialize f with (τ := τ').
-      apply f. right; apply hasτ'.
-  - destruct h as [h | h]; subst.
-    + pose proof f τ₁ (inl eq_refl) as h.
-      destruct h as [h | h]; subst.
-      * left; reflexivity.
-      * right. apply ih.
-        intros τ hτ.
-        pose proof f _ (inr hτ) as h'.
-        destruct h' as [h' | h']; subst.
-        -- 
-      
+  intros Δ Γ₁ Γ₂ f τ h.
+  apply map_has in h as [τ' τ'eq h]; subst.
+  apply has_map,f,h.
+Defined.
+          
 Equations Rename : forall {Δ : nat} {Γ₁ Γ₂ : list (type Δ)},
     (forall τ : type Δ, Has τ Γ₁ -> Has τ Γ₂) ->
     forall {τ : type Δ}, Γ₁ ⊢ τ -> Γ₂ ⊢ τ :=
   Rename ρ (Id _ _ has) := Id _ _ (ρ _ has);
   Rename ρ (λ σ ⇒ t)%term := (λ σ ⇒ Rename (ext' ρ σ) t)%term;
   Rename ρ (t₁ ⋅ t₂)%term := (Rename ρ t₁ ⋅ Rename ρ t₂)%term;
-  Rename ρ (Λ t)%term     := (Λ Rename _ t)%term;
+  Rename ρ (Λ t)%term     := (Λ Rename (S_Renamer ρ) t)%term;
   Rename ρ (t ⦗ τ ⦘)%term := ((Rename ρ t) ⦗ τ ⦘)%term.
+
+Definition exts : forall {Δ : nat} {Γ₁ Γ₂ : list (type Δ)},
+    (forall τ : type Δ, Has τ Γ₁ -> Γ₂ ⊢ τ) ->
+    forall (ρ τ : type Δ), Has τ (ρ :: Γ₁) -> ρ :: Γ₂ ⊢ τ.
+Proof.
+  cbn; intros Δ Γ₁ Γ₂ σ ρ τ [h | h]; subst.
+  - refine (Id _ τ _); cbn; left; reflexivity.
+  - refine (Rename _ (σ _ h)).
+    intros α has; cbn; right; exact has.
+Defined.
+
+Definition S_subs : forall {Δ : nat} {Γ₁ Γ₂ : list (type Δ)},
+    (forall τ : type Δ, Has τ Γ₁ -> Γ₂ ⊢ τ) ->
+    forall (τ : type (S Δ)), Has τ (map S_type Γ₁) -> map S_type Γ₂ ⊢ τ.
+Proof.
+  intros Δ Γ₁ Γ₂ σ τ h.
+  apply map_has in h as [τ' ? h]; subst.
+  apply σ in h.
+  apply S_term, h.
+Defined.
+
+Equations subs : forall {Δ : nat} {Γ₁ Γ₂ : list (type Δ)},
+    (forall τ : type Δ, Has τ Γ₁ -> Γ₂ ⊢ τ) ->
+    forall {τ : type Δ}, Γ₁ ⊢ τ -> Γ₂ ⊢ τ :=
+  subs σ (Id _ _ h)     := σ _ h;
+  subs σ (λ τ ⇒ t)%term := (λ τ ⇒ subs (exts σ τ) t)%term;
+  subs σ (t₁ ⋅ t₂)%term := (subs σ t₁ ⋅ subs σ t₂)%term;
+  subs σ (Λ t)%term     := (Λ subs (S_subs σ) t)%term;
+  subs σ (t ⦗ τ ⦘)%term := (subs σ t ⦗ τ ⦘)%term.
